

2DE/2DE3 Example sheet 3 solutions: Power series solutions of ODEs

1. Find the intervals of convergence of

(a)

$$\sum_{n=0}^{\infty} \frac{3^n}{n!} x^n,$$

We can use the Ratio Test:

$$\begin{aligned} L &= \lim_{n \rightarrow \infty} \left| \frac{3^{n+1}}{(n+1)!} x^{n+1} \frac{n!}{3^n x^n} \right|, \\ &= |x| \lim_{n \rightarrow \infty} \left| \frac{3}{n+1} \right|, \\ &= |x| \lim_{n \rightarrow \infty} \left(\frac{\frac{3}{n}}{1 + \frac{1}{n}} \right), \\ &= 0. \end{aligned}$$

Hence, $L < 1$ for all x and the interval of convergence is $(-\infty, \infty)$.

(b)

$$\sum_{n=0}^{\infty} \frac{n^2}{2^n} (x+2)^n.$$

We again use the Ratio Test:

$$\begin{aligned} L &= \lim_{n \rightarrow \infty} \left| \frac{(n+1)^2 (x+2)^{n+1} 2^n}{2^{n+1} n^2 (x+2)^n} \right|, \\ &= |x+2| \lim_{n \rightarrow \infty} \left(\frac{(n+1)^2}{2n^2} \right), \\ &= |x+2| \lim_{n \rightarrow \infty} \left(\frac{n^2 + 2n + 1}{2n^2} \right), \\ &= |x+2| \lim_{n \rightarrow \infty} \left(\frac{1 + \frac{2}{n} + \frac{1}{n^2}}{2} \right), \\ &= \frac{1}{2} |x+2|. \end{aligned}$$

Therefore the series converges if

$$\begin{aligned} \frac{1}{2} |x+2| &< 1, \\ |x+2| &< 2, \\ -2 &< x+2 < 2, \\ -4 &< x < 0. \end{aligned}$$

We also need to check what happens when $\frac{1}{2}|x+2| = 1$. This happens if $x = 0$ or $x = -4$.

If $x = 0$,

$$\sum_{n=0}^{\infty} \frac{n^2}{2^n} (x+2)^n = \sum_{n=0}^{\infty} n^2,$$

and this diverges.

If $x = -4$,

$$\sum_{n=0}^{\infty} \frac{n^2}{2^n} (x+2)^n = \sum_{n=0}^{\infty} \frac{n^2}{2^n} (-2)^n = \sum_{n=0}^{\infty} (-1)^n n^2,$$

and this diverges (the individual terms do not tend to zero).

Therefore, the interval of convergence is $(-4, 0)$.

2. *Let*

$$f(x) = \sum_{n=0}^{\infty} \frac{1}{n+1} x^n \quad \text{and} \quad g(x) = \sum_{n=1}^{\infty} 2^{-n} x^{n-1}.$$

Find $f(x) + g(x)$ as a power series with a single sum.

We first rewrite $g(x)$ as a series from $n = 0$, i.e. $n' = n - 1 \iff n = n' + 1$:

$$\begin{aligned} g(x) &= \sum_{n'=0}^{\infty} 2^{-(n'+1)} x^{n'}, \\ &= \sum_{n=0}^{\infty} 2^{-(n+1)} x^n \quad (\text{dropping primes}). \end{aligned}$$

Therefore,

$$\begin{aligned} f(x) + g(x) &= \sum_{n=0}^{\infty} \frac{1}{n+1} x^n + 2^{-(n+1)} x^n, \\ &= \sum_{n=0}^{\infty} \left(\frac{1}{n+1} + 2^{-(n+1)} \right) x^n. \end{aligned}$$

3. *Find $f'(x)$ and $g'(x)$ given*

(a)

$$f(x) = \sum_{n=0}^{\infty} (-1)^n x^n,$$

$$f'(x) = \sum_{n=0}^{\infty} (-1)^n n x^{n-1},$$

which is the same as

$$\sum_{n=1}^{\infty} (-1)^n n x^{n-1}.$$

(b)

$$g(x) = \sum_{n=0}^{\infty} \frac{(-1)^n}{(2n+1)!} x^{2n+1}.$$

$$\begin{aligned} g'(x) &= \sum_{n=0}^{\infty} \frac{(-1)^n (2n+1)}{(2n+1)!} x^{2n}, \\ &= \sum_{n=0}^{\infty} \frac{(-1)^n}{(2n)!} x^{2n}. \end{aligned}$$

4. In the above example, the series given by $f(x)$ and $g(x)$ converge to $f(x) = (1+x)^{-1}$ and $g(x) = \sin(x)$ (you can check this by deriving the Taylor series of these functions and showing that they are the same as the series above). Verify therefore that your answers for $f'(x)$ and $g'(x)$ are correct by differentiating $f(x) = (1+x)^{-1}$ and $g(x) = \sin(x)$ directly and calculating the first few terms of the Taylor series of $f'(x)$ and $g'(x)$ about $x = 0$.

(a)

$$\begin{aligned} f(x) &= (1+x)^{-1}, \\ f'(x) &= -(1+x)^{-2} = F(x), \\ f''(x) &= 2(1+x)^{-3} = F'(x), \\ f'''(x) &= -6(1+x)^{-4} = F''(x), \\ &\vdots \end{aligned}$$

Therefore the Taylor series for $f'(x) = F(x)$ is given by

$$\begin{aligned} F(x) &= F(0) + F'(0)x + \frac{F''(0)}{2!}x^2 + \dots \\ &= -1 + 2x - 3x^2 + \dots \\ &= \sum_{n=0}^{\infty} (-1)^n n x^{n-1}. \end{aligned}$$

(b)

$$\begin{aligned}
g(x) &= \sin(x), \\
g'(x) &= \cos(x) = G(x), \\
g''(x) &= -\sin(x) = G'(x), \\
g'''(x) &= -\cos(x) = G''(x), \\
&\vdots
\end{aligned}$$

Therefore the Taylor series for $g'(x) = G(x)$ is given by

$$\begin{aligned}
G(x) &= G(0) + G'(0)x + \frac{G''(0)}{2!}x^2 + \dots \\
&= 1 - \frac{x^2}{2} + \frac{x^4}{24} - \dots \\
&= \sum_{n=0}^{\infty} \frac{(-1)^n}{(2n)!} x^{2n}.
\end{aligned}$$

5. Rewrite the following as sums from $n = 0$ and simplify the resulting series wherever possible:

(a)

$$\sum_{n=2}^{\infty} n(n-1)a_n x^{n-2},$$

Let $n' = n - 2 \iff n = n' + 2$, then

$$\begin{aligned}
\sum_{n=2}^{\infty} n(n-1)a_n x^{n-2} &= \sum_{n'=0}^{\infty} (n'+2)(n'+1)a_{n'+2} x^{n'}, \\
&= \sum_{n=0}^{\infty} (n+2)(n+1)a_{n+2} x^n.
\end{aligned}$$

(b)

$$\sum_{m=2}^{\infty} m(m-1)a_m x^{m-2} + x \sum_{k=1}^{\infty} k a_k x^{k-1}.$$

$$\begin{aligned}
\sum_{m=2}^{\infty} m(m-1)a_mx^{m-2} + x \sum_{k=1}^{\infty} ka_kx^{k-1} &= \sum_{m=2}^{\infty} m(m-1)a_mx^{m-2} + \sum_{k=1}^{\infty} ka_kx^k, \\
&= \sum_{m=2}^{\infty} m(m-1)a_mx^{m-2} + \sum_{k=0}^{\infty} ka_kx^k, \\
&= \sum_{m'=0}^{\infty} (m+2)(m+1)a_{m+2}x^m + \sum_{k=0}^{\infty} ka_kx^k \\
&\quad \text{(using } m' = m - 2 \iff m = m' + 2), \\
&= \sum_{n=0}^{\infty} (n+2)(n+1)a_{n+2}x^n + na_nx^n, \\
&= \sum_{n=0}^{\infty} [(n+2)(n+1)a_{n+2} + na_n]x^n.
\end{aligned}$$

6. Find the Taylor series of $f(x)$ around $x = x_0$ for the following functions and determine the interval of convergence in each case.

(a)

$$f(x) = e^x, \quad x_0 = 0$$

$$\begin{aligned}
f(x) &= e^x, \\
&= \sum_{n=0}^{\infty} \frac{x^n}{n!}.
\end{aligned}$$

Then the Ratio Test gives:

$$\begin{aligned}
L &= \lim_{n \rightarrow \infty} \left| \frac{x^{n+1}}{(n+1)!} \frac{n!}{x^n} \right|, \\
&= |x| \lim_{n \rightarrow \infty} \left(\frac{1}{n+1} \right), \\
&= 0
\end{aligned}$$

for all x so the interval of convergence is $(-\infty, \infty)$.

(b)

$$f(x) = \ln(x), \quad x_0 = 1.$$

$$\begin{aligned}
f(x - x_0) &= f(x_0) + (x - x_0)f'(x_0) + \frac{(x - x_0)^2}{2!}f''(x_0) + \frac{(x - x_0)^3}{3!}f'''(x_0) + \dots \\
\implies f(x - 1) &= 0 + (x - 1) - \frac{(x - 1)^2}{2} + \frac{(x - 1)^3}{3} + \dots, \\
&= \sum_{n=1}^{\infty} \frac{(-1)^{n+1}(x - 1)^n}{n}.
\end{aligned}$$

Then the Ratio Test gives:

$$\begin{aligned} L &= \lim_{n \rightarrow \infty} \left| \frac{(-1)^{n+2}(x-1)^{n+1}}{n+1} \frac{n}{(-1)^{n+1}(x-1)^n} \right|, \\ &= |x-1| \lim_{n \rightarrow \infty} \left(\frac{n}{n+1} \right), \\ &= |x-1|. \end{aligned}$$

This series therefore converges if

$$\begin{aligned} |x-1| &< 1, \\ -1 &< x-1 < 1, \\ 0 &< x < 2. \end{aligned}$$

We also need to check what happens when $|x-1| = 1$, i.e. $x = 0, 2$.

If $x = 0$,

$$\begin{aligned} f(0-1) &= f(-1), \\ &= \sum_{n=1}^{\infty} \frac{(-1)^{n+1}(-1)^n}{n}, \\ &= \sum_{n=1}^{\infty} \frac{(-1)^{2n+1}}{n}, \\ &= \sum_{n=1}^{\infty} -\frac{1}{n}, \end{aligned}$$

which diverges.

If $x = 2$,

$$\begin{aligned} f(2-1) &= f(1), \\ &= \sum_{n=1}^{\infty} \frac{(-1)^{n+1}(1)^n}{n}, \\ &= \sum_{n=1}^{\infty} \frac{(-1)^{n+1}}{n}, \end{aligned}$$

which converges.

Therefore the interval of convergence is $(0, 2]$.

7. Determine the a_n (in terms of a_0) such that

$$\sum_{n=1}^{\infty} n a_n x^{n-1} + 2 \sum_{n=0}^{\infty} a_n x^n = 0,$$

is satisfied.

To shift the sums so that both sums are in terms of x^n , let $n = n' + 1 \iff n' = n - 1$

in the first sum. Then the above is equivalent to

$$\sum_{n=0}^{\infty} (n+1)a_{n+1}x^n + 2 \sum_{n=0}^{\infty} a_n x^n = 0,$$

$$\sum_{n=0}^{\infty} [(n+1)a_{n+1} + 2a_n]x^n = 0.$$

Matching coefficients of x^n gives us

$$(n+1)a_{n+1} = -2a_n,$$

$$a_{n+1} = \frac{-2}{n+1}a_n.$$

This will generate the coefficients

$$a_{n+1} = \frac{(-2)^{n+1}}{(n+1)!}a_0 \quad \text{or} \quad a_n = \frac{(-2)^n}{n!}a_0.$$

8. Show that the power series solution about $x = 0$ to

$$2y'' + (x+1)y' + y = 0$$

is given by

$$y = a_0 \left(1 - \frac{x^2}{4} + \frac{x^3}{24} + \dots \right) + a_1 \left(x - \frac{x^2}{4} - \frac{x^3}{8} + \dots \right),$$

where a_0 and a_1 are constants.

Because $x = 0$ is an ordinary point of the equation, we look for a solution in the form

$$y = \sum_{n=0}^{\infty} a_n x^n,$$

$$\Rightarrow y' = \sum_{n=1}^{\infty} n a_n x^{n-1},$$

$$y'' = \sum_{n=2}^{\infty} n(n-1) a_n x^{n-2}.$$

Substituting these into the equation gives

$$2 \sum_{n=2}^{\infty} n(n-1) a_n x^{n-2} + (x+1) \sum_{n=1}^{\infty} n a_n x^{n-1} + \sum_{n=0}^{\infty} a_n x^n = 0,$$

$$\sum_{n=2}^{\infty} 2n(n-1) a_n x^{n-2} + \sum_{n=1}^{\infty} n a_n x^n + \sum_{n=1}^{\infty} n a_n x^{n-1} + \sum_{n=0}^{\infty} a_n x^n = 0.$$

Shift the indices of the sums so that all are in terms of powers of x^n , i.e. let

$n' = n - 2 \iff n = n' + 2$ in the first sum and $n^* = n - 1 \iff n = n^* + 1$ in the third sum to give

$$\begin{aligned} \sum_{n'=0}^{\infty} 2(n'+2)(n'+1)a_{n'+2}x^n + \sum_{n=1}^{\infty} na_nx^n + \sum_{n^*=0}^{\infty} (n^*+1)a_{n^*+1}x^{n^*} + \sum_{n=0}^{\infty} a_nx^n &= 0, \\ \sum_{n=0}^{\infty} 2(n+2)(n+1)a_{n+2}x^n + \sum_{n=0}^{\infty} na_nx^n + \sum_{n=0}^{\infty} (n+1)a_{n+1}x^n + \sum_{n=0}^{\infty} a_nx^n &= 0 \\ &\text{(dropping ' and *)}. \end{aligned}$$

(Note that in the second sum we can shift the start point to $n = 0$). Then gather the sums into one:

$$\begin{aligned} \sum_{n=0}^{\infty} [2(n+2)(n+1)a_{n+2} + na_n + (n+1)a_{n+1} + a_n]x^n &= 0, \\ \sum_{n=0}^{\infty} [2(n+2)(n+1)a_{n+2} + (n+1)a_{n+1} + (n+1)a_n]x^n &= 0. \end{aligned}$$

Matching coefficients of x^0 (i.e. looking at $n = 0$):

$$\begin{aligned} 2 \times 2 \times 1a_2 + a_1 + a_0 &= 0, \\ 4a_2 + a_1 + a_0 &= 0, \\ a_2 &= -\frac{(a_1 + a_0)}{4}. \end{aligned}$$

Matching the coefficients of x (i.e. looking at $n = 1$):

$$\begin{aligned} 2 \times 3 \times 2a_3 + 2a_2 + 2a_1 &= 0, \\ a_3 &= -\frac{(a_2 + a_1)}{6}, \\ &= -\frac{1}{6} \left(-\frac{(a_1 + a_0)}{4} + a_1 \right), \\ &= \frac{a_1 + a_0}{24} - \frac{a_1}{6}, \\ &= \frac{-3a_1 + a_0}{24}. \end{aligned}$$

$$\begin{aligned} \implies y &= \sum_{n=0}^{\infty} a_nx^n, \\ &= a_0 + a_1x - \left(\frac{a_1 + a_0}{4} \right) x^2 + \left(\frac{-3a_1 + a_0}{24} \right) x^3 + \dots, \\ &= a_0 \left(1 - \frac{x^2}{4} + \frac{x^3}{24} + \dots \right) + a_1 \left(x - \frac{x^2}{4} - \frac{x^3}{8} + \dots \right). \end{aligned}$$

9. Show that the power series solution about $x = 1$ to

$$(x^2 - 2x)y'' + 2y = 0$$

is given by

$$y = a_0 \left(1 + (x-1)^2 + \frac{(x-1)^4}{3} + \dots \right) + a_1 \left((x-1) + \frac{(x-1)^3}{3} + \frac{2(x-1)^5}{15} + \dots \right),$$

where a_0 and a_1 are constants. [Hint: express $x^2 - 2x$ in terms of $x - 1$]. Use the Ratio Test on the recurrence relation to show that the series converges in an interval around $x = 1$.

Because $x = 1$ is an ordinary point of the equation, we look for a solution in the form

$$\begin{aligned} y &= \sum_{n=0}^{\infty} a_n (x-1)^n, \\ \Rightarrow y' &= \sum_{n=1}^{\infty} a_n n (x-1)^{n-1}, \\ y'' &= \sum_{n=2}^{\infty} n(n-1) a_n (x-1)^{n-2}. \end{aligned}$$

Substitute these into the equation:

$$\begin{aligned} (x^2 - 2x) \sum_{n=2}^{\infty} n(n-1) a_n (x-1)^{n-2} + 2 \sum_{n=0}^{\infty} a_n (x-1)^n &= 0, \\ [(x-1)^2 - 1] \sum_{n=2}^{\infty} n(n-1) a_n (x-1)^{n-2} + 2 \sum_{n=0}^{\infty} a_n (x-1)^n &= 0, \\ \sum_{n=2}^{\infty} n(n-1) a_n (x-1)^n - \sum_{n=2}^{\infty} n(n-1) a_n (x-1)^{n-2} + \sum_{n=0}^{\infty} 2a_n (x-1)^n &= 0, \\ \sum_{n=2}^{\infty} n(n-1) a_n (x-1)^n - \sum_{n=0}^{\infty} (n+2)(n+1) a_{n+2} (x-1)^n + \sum_{n=0}^{\infty} 2a_n (x-1)^n &= 0, \\ \sum_{n=0}^{\infty} [n(n-1) a_n - (n+2)(n+1) a_{n+2} + 2a_n] (x-1)^n &= 0, \\ \sum_{n=0}^{\infty} [(n(n-1) + 2) a_n - (n+2)(n+1) a_{n+2}] (x-1)^n &= 0. \end{aligned}$$

Match the coefficients of $(x-1)^n$:

$$\begin{array}{ll}
 n = 0, & 2a_0 - 2a_2 = 0 \implies a_2 = a_0, \\
 n = 1, & 2a_1 - 6a_3 = 0 \implies a_3 = \frac{a_1}{3}, \\
 n = 2, & 4a_2 - 12a_4 = 0 \implies a_4 = \frac{a_2}{3} = \frac{a_0}{3}, \\
 n = 3, & 8a_3 - 20a_5 = 0 \implies a_5 = \frac{2a_3}{5} = \frac{2a_1}{15}, \\
 \vdots & \vdots
 \end{array}$$

Hence

$$y = a_0 \left(1 + (x-1)^2 + \frac{(x-1)^4}{3} + \dots \right) + a_1 \left((x-1) + \frac{(x-1)^3}{3} + \frac{2(x-1)^5}{15} + \dots \right).$$

In general,

$$\begin{aligned}
 a_{n+2} &= \frac{(n(n-1)+2)}{(n+2)(n+1)} a_n, \\
 &= \frac{n^2 - n + 2}{n^2 + 3n + 2} a_n,
 \end{aligned}$$

and we can use this to check that the series converge by the Ratio Test:

$$\begin{aligned}
 L &= \lim_{n \rightarrow \infty} \left| \frac{a_{n+2}(x-1)^{n+2}}{a_n(x-1)^n} \right|, \\
 &= (x-1)^2 \lim_{n \rightarrow \infty} \left| \frac{n^2 - n + 2}{n^2 + 3n + 2} \right|, \\
 &= (x-1)^2 \lim_{n \rightarrow \infty} \left| \frac{1 - \frac{1}{n} + \frac{2}{n^2}}{1 + \frac{3}{n} + \frac{2}{n^2}} \right|, \\
 &= (x-1)^2.
 \end{aligned}$$

Hence the series converge if

$$\begin{aligned}
 (x-1)^2 &< 1, \\
 -1 &< x-1 < 1, \\
 0 &< x < 2.
 \end{aligned}$$

This confirms that both series should converge in an interval around $x = 1$.

10. Find the solution of the previous question if $y(1) = 2$ and $y'(1) = 4$.

$$\begin{aligned}
 y(1) &= a_0 = 2, \\
 y'(1) &= a_1 = 4.
 \end{aligned}$$

is given by

$$y = - \left(x - \frac{x^3}{3} - \frac{x^4}{12} + \dots \right).$$

[Hint: can you express e^x as a power series?]

First we need to express e^x as a power series. We use its Taylor series expansion for this:

$$\begin{aligned} f(x) &= f(0) + f'(0)x + \frac{f''(0)}{2!}x^2 + \frac{f'''(0)}{3!}x^3 + \dots \\ \implies e^x &= 1 + x + \frac{x^2}{2!} + \frac{x^3}{3!} + \dots \\ &= \sum_{n=0}^{\infty} \frac{x^n}{n!}. \end{aligned}$$

Then substituting this and $y = \sum_{n=0}^{\infty} a_n x^n$ ($x = 0$ is an ordinary point) into our equation, we have

$$\sum_{n=2}^{\infty} n(n-1)a_n x^{n-2} + \sum_{n=1}^{\infty} n a_n x^n + \sum_{n=0}^{\infty} \frac{x^n}{n!} \sum_{n=0}^{\infty} a_n x^n = 0.$$

To handle the multiplicative term, it's easiest to write out the first few terms in each sum, e.g.

$$\begin{aligned} &2a_2 + 6a_3x + 12a_4x^2 + 20a_5x^3 + \dots \\ &+ a_1x + 2a_2x^2 + 3a_3x^3 + 4a_4x^4 + \dots \\ &+ \left(1 + x + \frac{x^2}{2} + \frac{x^3}{6} + \dots \right) (a_0 + a_1x + a_2x^2 + a_3x^3 + \dots) = 0. \end{aligned}$$

Then, matching coefficients we have:

$$\begin{aligned} x^0 : \quad &2a_2 + a_0 = 0 \implies a_2 = -\frac{a_0}{2}, \\ x^1 : \quad &6a_3 + a_1 + a_1 + a_0 = 0 \implies 6a_3 + 2a_1 + a_0 = 0 \implies a_3 = -\frac{a_1}{3} - \frac{a_0}{6}, \\ x^2 : \quad &12a_4 + 2a_2 + a_2 + a_1 + \frac{a_0}{2} = 0 \implies 12a_4 + 3a_2 + a_1 + \frac{a_0}{2} = 0 \\ &\implies a_4 = \frac{-1}{12} \left(3a_2 + a_1 + \frac{a_0}{2} \right) = \frac{a_0}{12} - \frac{a_1}{12}, \\ x^3 : \quad &20a_5 + 3a_3 + a_3 + a_2 + \frac{a_1}{2} + \frac{a_0}{6} = 0 \implies 20a_5 = - \left(4a_3 + a_2 + \frac{a_1}{2} + \frac{a_0}{6} \right), \end{aligned}$$

etc.

This gives us

$$y = a_0 \left(1 - \frac{x^2}{2} - \frac{x^3}{6} + \frac{x^4}{12} + \dots \right) + a_1 \left(x - \frac{x^3}{3} - \frac{x^4}{12} + \dots \right).$$

Imposing the initial conditions tells us

$$\begin{aligned}y(0) &= a_0 = 0, \\y'(0) &= a_1 = -1,\end{aligned}$$

so that

$$y = -\left(x - \frac{x^3}{3} - \frac{x^4}{12} + \dots\right).$$

13. Show that the power series solution about $x = 0$ to

$$(x+2)x^2y'' - xy' + (1+x)y = 0, \quad x > 0,$$

is given by

$$y = \alpha_1 \left(x - \frac{x^2}{3} + \frac{x^3}{10} - \frac{x^4}{30} + \dots\right) + \alpha_2 \left(x^{\frac{1}{2}} - \frac{3x^{\frac{3}{2}}}{4} + \frac{7x^{\frac{5}{2}}}{32} - \frac{133x^{\frac{7}{2}}}{1920} + \dots\right),$$

where α_1 and α_2 are constants.

We first need to check whether $x = 0$ is an ordinary point or a singular point. Rearranging the equation into the standard form, we have:

$$y'' - \frac{1}{x(x+2)}y' + \frac{(1+x)}{x^2(x+2)}y = 0,$$

so that

$$\begin{aligned}p(x) &= \frac{-1}{x(x+2)} \implies xp(x) = \frac{-1}{x+2}, \\q(x) &= \frac{1+x}{x^2(x+2)} \implies x^2q(x) = \frac{1+x}{x+2}.\end{aligned}$$

Neither $p(x)$ nor $q(x)$ are analytic at $x = 0$ so this is a singular point. However, both $xp(x)$ and $x^2q(x)$ are analytic at $x = 0$ therefore this is a regular singular point, so we must look for a solution in the form

$$\begin{aligned}y &= \sum_{n=0}^{\infty} a_n x^{n+r}, \\ \implies y' &= \sum_{n=0}^{\infty} a_n (n+r) x^{n+r-1}, \\ y'' &= \sum_{n=0}^{\infty} a_n (n+r)(n+r-1) x^{n+r-2}.\end{aligned}$$

It is now easier to proceed with the original equation, rather than the standard form. Thus, substituting the above into the original equation gives

$$\begin{aligned} (x+2)x^2 \sum_{n=0}^{\infty} a_n(n+r)(n+r-1)x^{n+r-2} - x \sum_{n=0}^{\infty} a_n(n+r)x^{n+r-1} + (1+x) \sum_{n=0}^{\infty} a_n x^{n+r} = 0, \\ \sum_{n=0}^{\infty} a_n(n+r)(n+r-1)x^{n+r+1} + \sum_{n=0}^{\infty} 2a_n(n+r)(n+r-1)x^{n+r} - \sum_{n=0}^{\infty} a_n(n+r)x^{n+r} \\ + \sum_{n=0}^{\infty} a_n x^{n+r} + \sum_{n=0}^{\infty} a_n x^{n+r+1} = 0. \end{aligned}$$

We next want all sums to be in terms of x^{n+r} , so let $n' = n+1$ in the first and final sums (and drop primes):

$$\begin{aligned} \sum_{n=1}^{\infty} a_{n-1}(n+r-1)(n+r-2)x^{n+r} + \sum_{n=0}^{\infty} 2a_n(n+r)(n+r-1)x^{n+r} - \sum_{n=0}^{\infty} a_n(n+r)x^{n+r} \\ + \sum_{n=0}^{\infty} a_n x^{n+r} + \sum_{n=1}^{\infty} a_{n-1}x^{n+r} = 0. \end{aligned}$$

Next, for the middle three sums, take the $n=0$ terms outside their sums so that all sums can then be combined:

$$\begin{aligned} 2a_0r(r-1)x^r - a_0rx^r + a_0x^r \\ + \sum_{n=1}^{\infty} (a_{n-1}(n+r-1)(n+r-2) + 2a_n(n+r)(n+r-1) - a_n(n+r) + a_n + a_{n-1})x^{n+r} = 0, \\ [2r(r-1) - r + 1]a_0x^r \\ + \sum_{n=1}^{\infty} [(n+r-1)(n+r-2) + 1]a_{n-1} + (2(n+r)(n+r-1) - (n+r) + 1)a_n]x^{n+r} = 0. \end{aligned}$$

Setting the coefficients of x^r to be zero to match the RHS we see that $2r^2 - 3r + 1 = 0$, i.e. $r = 1$ or $r = \frac{1}{2}$.

Setting the coefficients of x^{n+r} to be zero gives

$$\begin{aligned} a_n &= -\frac{(n+r-1)(n+r-2) + 1}{2(n+r)(n+r-1) - (n+r) + 1} a_{n-1}, \\ &= -\frac{(n+r-1)(n+r-2) + 1}{(n+r-1)(2(n+r) - 1)} a_{n-1}, \\ &= -\frac{(n+r-1)(n+r-2) + 1}{(n+r-1)(2n+2r-1)} a_{n-1}. \end{aligned}$$

Let $r = 1$, then

$$\begin{aligned} a_1 &= \frac{-a_0}{3}, \\ a_2 &= \frac{-3a_1}{10} = \frac{a_0}{10}, \\ a_3 &= \frac{-7a_2}{21} = \frac{-7}{21} \left(\frac{a_0}{10} \right) = \frac{-a_0}{30}, \\ &\vdots \end{aligned}$$

Let $r = \frac{1}{2}$, then

$$\begin{aligned} a_1 &= \frac{-3a_0}{4}, \\ a_2 &= \frac{-\frac{7}{4}a_1}{6} = \frac{7a_0}{32}, \\ a_3 &= \frac{-\frac{19}{4}a_2}{15} = \frac{-133a_0}{1920}, \\ &\vdots \end{aligned}$$

Hence,

$$\begin{aligned} y &= \alpha_1 x \left(1 - \frac{x}{3} + \frac{x^2}{10} - \frac{x^3}{30} + \dots \right) + \alpha_2 x^{\frac{1}{2}} \left(1 - \frac{3x}{4} + \frac{7x^2}{32} - \frac{133x^3}{1920} + \dots \right), \\ &= \alpha_1 \left(x - \frac{x^2}{3} + \frac{x^3}{10} - \frac{x^4}{30} + \dots \right) + \alpha_2 \left(x^{\frac{1}{2}} - \frac{3x^{\frac{3}{2}}}{4} + \frac{7x^{\frac{5}{2}}}{32} - \frac{133x^{\frac{7}{2}}}{1920} + \dots \right). \end{aligned}$$

Notice that we must replace a_0 with α_1 and α_2 because the a_0 in the two series may differ.

14. Show that the power series solution about $x = 0$ to

$$3x^2y'' + 2xy' + x^2y = 0, \quad x > 0,$$

is given by

$$y = \alpha_1 x^{\frac{1}{3}} \left(1 - \frac{x^2}{14} + \frac{x^4}{728} + \dots \right) + \alpha_2 \left(1 - \frac{x^2}{10} + \frac{x^4}{440} + \dots \right),$$

where α_1 and α_2 are constants.

We first need to check whether $x = 0$ is an ordinary point or a singular point. Rearranging the equation into the standard form, we have:

$$y'' + \frac{2}{3x}y' + \frac{1}{3}y = 0,$$

so that

$$\begin{aligned} p(x) &= \frac{2}{3x} \implies xp(x) = \frac{2}{3}, \\ q(x) &= \frac{1}{3} \implies x^2q(x) = \frac{x^2}{3}. \end{aligned}$$

$p(x)$ is not analytic at $x = 0$ so this is a singular point. However, both $xp(x)$ and $x^2q(x)$ are analytic at $x = 0$ therefore this is a regular singular point, so we must look for a solution in the form

$$\begin{aligned} y &= \sum_{n=0}^{\infty} a_n x^{n+r}, \\ \implies y' &= \sum_{n=0}^{\infty} a_n (n+r) x^{n+r-1}, \\ y'' &= \sum_{n=0}^{\infty} a_n (n+r)(n+r-1) x^{n+r-2}. \end{aligned}$$

It is now easier to proceed with the original equation, rather than the standard form. Thus, substituting the above into the original equation gives

$$3x^2 \sum_{n=0}^{\infty} a_n(n+r)(n+r-1)x^{n+r-2} + 2x \sum_{n=0}^{\infty} a_n(n+r)x^{n+r-1} + x^2 \sum_{n=0}^{\infty} a_n x^{n+r} = 0,$$

$$\sum_{n=0}^{\infty} 3a_n(n+r)(n+r-1)x^{n+r} + \sum_{n=0}^{\infty} 2a_n(n+r)x^{n+r} + \sum_{n=0}^{\infty} a_n x^{n+r+2} = 0.$$

We next want all sums to be in terms of x^{n+r} , so let $n' = n + 2$ in the final sum (and drop primes):

$$\sum_{n=0}^{\infty} 3a_n(n+r)(n+r-1)x^{n+r} + \sum_{n=0}^{\infty} 2a_n(n+r)x^{n+r} + \sum_{n=2}^{\infty} a_{n-2}x^{n+r} = 0.$$

Next, take the $n = 0$ and $n = 1$ terms from the first and second sums outside the sum so that all sums can be combined:

$$3a_0r(r-1)x^r + 3a_1(r+1)rx^{r+1} + 2a_0rx^r + 2a_1(r+1)x^{r+1} + \sum_{n=2}^{\infty} (3a_n(n+r)(n+r-1) + 2a_n(n+r) + a_{n-2})x^{n+r} = 0.$$

Matching the coefficients of x^r :

$$\begin{aligned} 3a_0r(r-1) + 2a_0r &= 0, \\ 3r^2 - 3r + 2r &= 0 \quad (a_0 \neq 0), \\ 3r^2 - r &= 0, \\ r(3r-1) &= 0 \implies r = 0 \quad \text{or } r = \frac{1}{3}. \end{aligned}$$

Matching the coefficients of x^{r+1} when $r = 0$:

$$2a_1 = 0 \implies a_1 = 0.$$

Matching the coefficients of x^{r+1} when $r = \frac{1}{3}$:

$$3a_1 \left(\frac{4}{3}\right) \left(\frac{1}{3}\right) + 2a_1 \left(\frac{4}{3}\right) = 0 \implies 4a_1 = 0 \implies a_1 = 0.$$

Matching the coefficients of x^{n+r} for general r :

$$\begin{aligned} a_n &= \frac{-a_{n-2}}{3(n+r)(n+r-1) + 2(n+r)}, \\ &= \frac{-a_{n-2}}{(n+r)(3n+3r-1)}. \end{aligned}$$

Hence, $a_3 = a_5 = a_7 = \dots = 0$ for either value of r .

If $r = 0$,

$$\begin{aligned} a_2 &= \frac{-a_0}{2 \times 5} = \frac{-a_0}{10}, \\ a_4 &= \frac{-a_2}{4 \times 11} = \frac{-a_2}{44} = \frac{a_0}{440}, \\ &\vdots \end{aligned}$$

If $r = \frac{1}{3}$,

$$\begin{aligned} a_2 &= \frac{-a_0}{\frac{7}{3} \times 6} = \frac{-a_0}{14}, \\ a_4 &= \frac{-a_2}{\frac{13}{3} \times 12} = \frac{-a_2}{52} = \frac{a_0}{728}, \\ &\vdots \end{aligned}$$

Hence,

$$y = \alpha_1 x^{\frac{1}{3}} \left(1 - \frac{x^2}{14} + \frac{x^4}{728} + \dots \right) + \alpha_2 \left(1 - \frac{x^2}{10} + \frac{x^4}{440} + \dots \right)$$

Notice that, as in the previous question, we replace a_0 with α_1 and α_2 because the a_0 in the two series may differ.